LeroyCompilerVerificationCourse/Deadcode.lean
@@ -114,7 +114,7 @@ theorem fixpoint_upper_bound (F : IdentSet → IdentSet) (default : IdentSet) (F
       deadcode_fixpoint (fun x => L' ∪ (live c x)) default
 
 theorem live_upper_bound:
-  forall c L,
+  ∀ c L,
    (live c L) ⊆ ((fv_com c) ∪  L) := by
     intro c
     induction c
@@ -225,10 +225,10 @@ theorem live_while_charact (b : bexp) (c : com) (L L' : IdentSet)
   | .WHILE b c => .WHILE b (dce c (live (.WHILE b c) L))
 
 @[grind] def agree (L: IdentSet) (s1 s2: store) : Prop :=
-  forall x, x  ∈ L -> s1 x = s2 x
+  ∀ x, x  ∈ L -> s1 x = s2 x
 
 @[grind] theorem agree_mon:
-  forall L L' s1 s2,
+  ∀ L L' s1 s2,
   agree L' s1 s2 -> L ⊆ L' -> agree L s1 s2 := by
     intro L L' s1 s2 AG sub
     unfold agree at *
@@ -238,8 +238,8 @@ theorem live_while_charact (b : bexp) (c : com) (L L' : IdentSet)
     exact AG
 
 @[grind] theorem aeval_agree:
-  forall L s1 s2, agree L s1 s2 ->
-  forall a, (fv_aexp a) ⊆ L -> aeval s1 a = aeval s2 a := by
+  ∀ L s1 s2, agree L s1 s2 ->
+  ∀ a, (fv_aexp a) ⊆ L -> aeval s1 a = aeval s2 a := by
     intro L s1 s2 AG a
     induction a
     any_goals grind
@@ -289,7 +289,7 @@ theorem live_while_charact (b : bexp) (c : com) (L L' : IdentSet)
 
 theorem beval_agree:
   ∀ L s1 s2, agree L s1 s2 ->
-  forall b, (fv_bexp b) ⊆ L -> beval s1 b = beval s2 b := by
+  ∀ b, (fv_bexp b) ⊆ L -> beval s1 b = beval s2 b := by
     intro L s1 s2 AG b
     induction b
     any_goals grind
@@ -343,7 +343,7 @@ theorem beval_agree:
       grind
 
 theorem agree_update_live:
-  forall s1 s2 L x v,
+  ∀ s1 s2 L x v,
   agree (L.erase x) s1 s2 ->
   agree L (update x v s1) (update x v s2) := by
     intro s1 s2 L x v AG
@@ -359,7 +359,7 @@ theorem agree_update_live:
       grind
 
 theorem agree_update_dead:
-  forall s1 s2 L x v,
+  ∀ s1 s2 L x v,
   agree L s1 s2 -> ¬x ∈ L ->
   agree L (update x v s1) s2 := by
     intro s1 s2 L x v AG not
@@ -370,9 +370,9 @@ theorem agree_update_dead:
     by_cases x=y <;> grind
 
 theorem dce_correct_terminating:
-  forall s c s', cexec s c s' ->
-  forall L s1, agree (live c L) s s1 ->
-  exists s1', cexec s1 (dce c L) s1' /\ agree L s' s1' := by
+  ∀ s c s', cexec s c s' ->
+  ∀ L s1, agree (live c L) s s1 ->
+  ∃ s1', cexec s1 (dce c L) s1' /\ agree L s' s1' := by
     intro s c s' EXEC
     induction EXEC
     any_goals grind
@@ -381,19 +381,19 @@ theorem dce_correct_terminating:
       have := live_while_charact b c1 L  (live (com.WHILE b c1) L) (by grind)
       have : agree (live c1 (live (com.WHILE b c1) L)) s1 s4 := by
         apply agree_mon
-        . exact hyp
-        . grind
+        · exact hyp
+        · grind
       have ⟨ t1, ht1, ht2⟩ :=  a_ih (live (.WHILE b c1) L) s4 this
       have ⟨u1, hu1, hu2 ⟩ :=  a_ih2 L t1 ht2
       exists u1
       constructor
       rotate_right
-      . exact hu2
-      . apply cexec.cexec_while_loop
-        . have := beval_agree (live (com.WHILE b c1) L) s1 s4 hyp b (by grind)
+      · exact hu2
+      · apply cexec.cexec_while_loop
+        · have := beval_agree (live (com.WHILE b c1) L) s1 s4 hyp b (by grind)
           grind
-        . exact ht1
-        . grind
+        · exact ht1
+        · grind
     case cexec_assign s2 x a=>
       intro L s3 AG
       simp [live] at AG
@@ -401,19 +401,19 @@ theorem dce_correct_terminating:
       case neg notIn =>
         exists s3
         constructor
-        . grind [dce]
-        . simp [notIn] at AG
+        · grind [dce]
+        · simp [notIn] at AG
           exact @agree_update_dead s2 s3 L x (aeval s2 a) (by grind) notIn
       case pos isIn =>
         simp [isIn] at AG
         exists (update x (aeval s3 a) s3)
         constructor
-        . simp [dce, isIn]
+        · simp [dce, isIn]
           grind
-        . have subgoal : aeval s2 a = aeval s3 a := by
+        · have subgoal : aeval s2 a = aeval s3 a := by
             apply aeval_agree
-            . exact AG
-            . intro y mem
+            · exact AG
+            · intro y mem
               grind
           rw [subgoal]
           apply @agree_update_live
@@ -423,8 +423,8 @@ theorem dce_correct_terminating:
       simp [dce]
       have EQ : beval s2 b = beval s4 b := by
         apply beval_agree
-        . apply AG
-        . simp [live]
+        · apply AG
+        · simp [live]
           intro y mem
           grind
       by_cases beval s2 b = true
@@ -436,9 +436,9 @@ theorem dce_correct_terminating:
         have ⟨s5 , EX', AG' ⟩ := ih (by grind)
         exists s5
         constructor
-        . apply cexec.cexec_ifthenelse
+        · apply cexec.cexec_ifthenelse
           grind
-        . exact AG'
+        · exact AG'
       case neg isFalse =>
         simp [isFalse] at EXEC
         specialize ih L s4
@@ -447,16 +447,16 @@ theorem dce_correct_terminating:
         have ⟨s5 , EX', AG' ⟩ := ih (by grind)
         exists s5
         constructor
-        . apply cexec.cexec_ifthenelse
+        · apply cexec.cexec_ifthenelse
           grind
-        . exact AG'
+        · exact AG'
     case cexec_while_done s2 b c isFalse =>
       intro L s1 AG
       have ⟨ h1 , h2 , h3 ⟩ := live_while_charact b c L (live (com.WHILE b c) L) (by grind)
       have EQ : beval s2 b = beval s1 b := by
         apply beval_agree
-        . apply AG
-        . intro y mem
+        · apply AG
+        · intro y mem
           specialize h1 y mem
           exact h1
       exists s1
